First-cut version of deposit.

src/dafny/smart/DepositSmart.dfy
@@ -71,48 +71,64 @@ module DepositSmart {
 
         //  Ghost variables used for the correctness proof.
 
+        /** The number of values added to the tree. */
+        // ghost var count : nat 
+
         /** The (Merkle) tree that corresponds to the list of values added so far. */
         ghost var t : Tree<T>
 
         /** The value of the root of the tree. */
-        ghost var r : T
+        // ghost var r : T
 
         /** The list of values added so far. */
         ghost var values : seq<T> 
 
-        /** Path to current to the leaf of index count. */
+        /** Path to index of next available leaf. */
         ghost var p : seq<bit>
 
-        /** The values on the left siblings of current path. */
-        ghost var left : seq<T>
+        /** The values on the left siblings on p. */
+        // ghost var left : seq<T>
 
         /** Property to maintain. */
         predicate Valid()
             reads this
         {
             //  Height and sequences sizes
-            1 <= TREE_HEIGHT ==  height(t) == |branch| == |zero_h| == |left| == |p|
+            1 <= TREE_HEIGHT ==  height(t) == |branch| == |zero_h| == |p|
             //  tree is not full
             && count < power2(TREE_HEIGHT)
 
-            && |values| <= power2(TREE_HEIGHT) == |leavesIn(t)|
+            && |values| == count <= power2(TREE_HEIGHT) == |leavesIn(t)|
 
             //  t is the Merkle tree for the valuea added so far. 
-            && isMerkle(t, values, f, d)
-            //  The right siblings of the current path are all zeroes
-            && (forall i :: 0 <= i < |zero_h| && p[i] == 0 ==> 
-                    siblingValueAt(p, t, i + 1) == zero_h[i])
+            && isMerkle(t, values, f, d) && hasLeavesIndexedFrom(t, 0)
 
-            && (r == t.v)
+            && zero_h == zeroes(f, d, TREE_HEIGHT - 1)
+            && (forall i :: 0 <= i < |zero_h| ==> 
+                    zero_h[i] == defaultValue(f, d, height(t) - 1 - i)
+            )
+            //  The right siblings of the current path are all zeroes
+            && (forall i :: 0 <= i < |p| ==> 
+                    siblingValueAt(p, t, i + 1) == 
+                        if p[i] == 0 then
+                             zero_h[i]
+                        else 
+                            branch[i]
+            )
+
+            // && (r == t.v)
             //  Path is to current next free leaf.
-            && bitListToNat(p) == count
+            // && bitListToNat(p) == count
+            && p == natToBitList(count, TREE_HEIGHT)
+            // && nodeAt(p, t) == leavesIn(t)[count]
+            // && nodeAt(p, t).v == lastVal
 
             //  Branch has values of left siblings of current path
-            && (forall i :: 0 <= i < |branch| && p[i] == 1 ==> 
-                    siblingValueAt(p, t, i + 1) == branch[i])
+            // && (forall i :: 0 <= i < |branch| && p[i] == 1 ==> 
+            //         siblingValueAt(p, t, i + 1) == branch[i])
 
-            && (forall i :: 0 <= i < |left| && p[i] == 1 ==> 
-                    siblingValueAt(p, t, i + 1) == left[i])
+            // && (forall i :: 0 <= i < |left| && p[i] == 1 ==> 
+            //         siblingValueAt(p, t, i + 1) == left[i])
         }
 
         /**
@@ -135,98 +151,297 @@ module DepositSmart {
             //  The values that have been added is initially empty.
             values := [];
             //  possibly left could be left uninitialised
-            left := l;
+            // left := l;
             //  Path to the first available leaf at index 0.
             p := natToBitList2(0, h);
             bitToNatToBitsIsIdentity(0, h);
             valueIsZeroImpliesAllZeroes(natToBitList2(0, h));
+            leafAtPathIsIntValueOfPath(natToBitList2(0, h), buildMerkle([], h, fun, default), 0, 0);
 
             rightSiblingsOfLastPathAreDefault(natToBitList2(0, h), buildMerkle([], h, fun, default), 0, fun, 0, default);
             //  Initially r is value of f for all leaves equal to default.
-            r := defaultValue(fun, default, h);
+            // r := defaultValue(fun, default, h);
             //  Use lemma to prove that r == t.v
             allLeavesDefaultImplyRootNodeDefault(buildMerkle([], h, fun, default), fun, default);
         }
 
-        method get_deposit_root() returns (h_root: T) 
-            requires Valid();
-            ensures h_root == t.v 
+        
+        method dep(v : T) 
+            requires Valid()
+            requires count < power2(TREE_HEIGHT) - 1         
+
+            ensures 1 <= TREE_HEIGHT ==  height(t) == |branch| == |zero_h| == |p|
+            ensures values == old(values) + [v]
+            ensures 1 <= |values| <= power2(height(t))
+            ensures count == old(count) + 1
+            ensures exists i :: 0 <= i < |old(p)| && old(p)[i] == 0
+            ensures p == nextPath(old(p))
+
+            ensures isMerkle(t, values, f, d) && hasLeavesIndexedFrom(t, 0)
+            ensures p == natToBitList(count, TREE_HEIGHT)
+            ensures count < power2(TREE_HEIGHT)
+            ensures |values| == count <= power2(TREE_HEIGHT) == |leavesIn(t)|
+
+            ensures zero_h == zeroes(f, d, TREE_HEIGHT - 1)
+            ensures (forall i :: 0 <= i < |p| ==> 
+                    siblingValueAt(p, t, i + 1) == 
+                        if p[i] == 0 then
+                             zero_h[i]
+                        else 
+                            branch[i])
+           
+            // ensures Valid()
+
+            modifies this 
         {
-            h_root := computeRootLeftRightUpWithIndex(TREE_HEIGHT, count, branch, zero_h, f, d);
+            t := buildMerkle(values + [v], TREE_HEIGHT, f, d);
+
+            nextPathSameSiblingsInNextList(TREE_HEIGHT, values, v, old(t), t, f, d, p);
+            assert(
+                reveal_siblingValueAt();
+                forall i :: 0 <= i < |p|  ==>
+                    siblingValueAt(p, t, i + 1) == siblingValueAt(p, old(t), i + 1)
+            );
+
+            assert(
+                reveal_siblingValueAt();
+                forall i :: 0 <= i < |p| ==> 
+                    siblingValueAt(p, t, i + 1) == 
+                    siblingValueAt(p, old(t), i + 1) == 
+                        if p[i] == 0 then
+                             zero_h[i]
+                        else 
+                            branch[i]
+            );
+
+            values := values + [v];
+
+            bitToNatToBitsIsIdentity(count, TREE_HEIGHT);
+            leafAtPathIsIntValueOfPath(p, t, count, 0);
+            
+            computeLeftSiblingOnNextPathFromLeftRightIsCorrectInATree(p, t, branch, zero_h, f, v, count);
+
+            assert(
+                forall i :: 0 <= i < |p| && nextPath(p)[i] == 1 ==> 
+                computeLeftSiblingOnNextPathFromLeftRight(p, branch, zero_h, f, v)[i] == siblingAt(take(nextPath(p), i + 1),t ).v
+            );
+
+            branch := computeLeftSiblingsOnNextpathWithIndex(TREE_HEIGHT, count, branch, zero_h, f, v);
+
+            bitToNatToBitsIsIdentity(count, TREE_HEIGHT);
+            pathToNoLasthasZero(p);
+            assert(exists i :: 0 <= i < |p| && p[i] == 0);
+
+            p := nextPath(p);
+
+            assert(count == old(count));
+            count := count + 1;
+            assert count == old(count) + 1;
+
+            pathToSucc(old(p), old(count), TREE_HEIGHT);
+
+            assert(
+                forall i :: 0 <= i < |p| && p[i] == 1 ==> 
+                    branch[i] == siblingAt(take(p, i + 1),t ).v
+            );
+
+            
+            assume(p == natToBitList(|values| - 1, TREE_HEIGHT));
+            assume(height(t) == TREE_HEIGHT);
+
+            // pathToLastInMerkleTreeHasZeroRightSiblings(p, values, t, f, d);
+            // assert(
+            //     // reveal_siblingValueAt();
+            //     forall i :: 0 <= i < |p| && p[i] == 0 ==> 
+            //         // siblingValueAt(p, t, i + 1) 
+            //         // siblingAt(take(p, i + 1),t ).v ==
+            //         zeroes(f, d, height(t) - 1)[i] 
+            //         == zero_h[i]
+            // );
+            forall ( i : nat | 0 <= i < |p| && p[i] == 0) 
+                // ensures siblingAt(take(p, i + 1),t ).v 
+                ensures siblingValueAt(p, t, i + 1) ==  zeroes(f, d, height(t) - 1)[i] 
+                // == zero_h[i]
+            {
+                //  reveal_siblingValueAt();
+                pathToLastInMerkleTreeHasZeroRightSiblings(p, values, t, f, d);
+            }
         }
+        
         /**
          *  Deposit a value i.e update the state.
          */
-        // method deposit(value : T) 
+        // method deposit(v : T) 
         //     requires Valid()
-        //     requires count < power2(TREE_HEIGHT) - 1
-
-        //     requires (forall i :: 0 <= i < |zeroes| && p[i] == 1 ==> 
-        //             siblingAt(take(p, i + 1), t).v == branch[i])
-
-        //     ensures Valid()
+        //     requires count < power2(TREE_HEIGHT) - 1 
             
-        //     modifies this
+        //     ensures 1 <= TREE_HEIGHT ==  height(t) == |branch| == |zero_h| == |left| == |p|
+        //     ensures count < power2(TREE_HEIGHT) 
+        //     ensures |values| == count < power2(TREE_HEIGHT) == |leavesIn(t)|
+        //     ensures isMerkle(t, values, f, d)
 
+        //     ensures p == natToBitList(old(count) + 1, TREE_HEIGHT)
+        //     ensures count == old(count) + 1
+        //     ensures p == natToBitList(count, TREE_HEIGHT)
+
+        //     // ensures (forall i :: 0 <= i < |p| && p[i] == 1 ==> 
+        //     //         siblingValueAt(p, t, i + 1) == branch[i]
+                        
+        //     // ensures nodeAt(p, t) == leavesIn(t)[count]
+
+        //     //  left siblings post condition
+
+
+        //     modifies this 
         // {
-        //     //   Update values
-        //     values := values[count := value];
-        //     //  Update tree
-        //     t := buildMerkle(values, TREE_HEIGHT, f, d);
-        //     //  The trees old(t) and t have same leaves except possibly at count
-        //     assert(take(leavesIn(old(t)), count) == take(leavesIn(t), count));
-        //     assert(drop(leavesIn(old(t)), count + 1) == drop(leavesIn(t), count + 1));
+        //     t := buildMerkle(values + [v], TREE_HEIGHT, f, d);
+        //     assert(hasLeavesIndexedFrom(t, 0));
+        //     assert(isCompleteTree(t));
+        //     bitToNatToBitsIsIdentity(old(count), TREE_HEIGHT) ;
+        //     bitToNatToBitsIsIdentity(count, TREE_HEIGHT) ;
+        //     assert( bitListToNat(old(p)) == old(count));
+        //     assert( bitListToNat(p) == count);
+        //     leafAtPathIsIntValueOfPath(p, t, count, 0);
+        //     leafAtPathIsIntValueOfPath(old(p), t, old(count), 0);
+        //     assert(nodeAt(old(p), t) == leavesIn(t)[old(count)]);
+        //     assert(nodeAt(p, t) == leavesIn(t)[count]);
+
+
+        //     nextPathSameSiblingsInNextList(TREE_HEIGHT, values, v, old(t), t, f, d, p);
+        //     assert(
+        //         reveal_siblingValueAt();
+        //         forall i :: 0 <= i < |p|  ==>
+        //             siblingValueAt(p, t, i + 1) == siblingValueAt(p, old(t), i + 1)
+        //     );
+
+        //     computeLeftSiblingOnNextPathFromLeftRightIsCorrectInATree(old(p), t, branch, zero_h, f, v, old(count));
+
+        //     // computeLeftSiblingOnNextPathFromLeftRightIsCorrectInATree(p, t, branch, zero_h, f, v, count);
+
+        //     // assert(
+        //     //     forall i :: 0 <= i < |old(p)| && nextPath(old(p))[i] == 1 ==> 
+        //     //     computeLeftSiblingOnNextPathFromLeftRight(old(p), branch, zero_h, f, v)[i] == siblingAt(take(nextPath(old(p)), i + 1),t ).v
+        //     // );
+
+        //     //  prove properties on left siblings.
+
+        //     values := values + [v];
+
+        //     //  before computing nextPath(p), prove bitListToNat(p) < power2(|p|) - 1
+        //     bitToNatToBitsIsIdentity(old(count), TREE_HEIGHT) ;
+        //     pathToNoLasthasZero(old(p));
+        //     assert(bitListToNat(old(p)) < power2(|old(p)|) - 1);
             
-           
-
-        //     bitToNatToBitsIsIdentity(count, TREE_HEIGHT);
-        //     assert(bitListToNat(p) == count < power2(TREE_HEIGHT) - 1);
-
-        //     //  the trees old(t) and t have same left siblings
-        //     //  they have similar values upto count.
-        // // requires drop(leavesIn(r), k + 1) == drop(leavesIn(r'), k + 1)
-        // assert(isCompleteTree(t));
-        // assert(isCompleteTree(old(t)));
-        // assert(isDecoratedWith(f, t));
-        // assert(isDecoratedWith(f, old(t)));
-        // assert(height(t) == height(old(t)) >= 1);
-        // assert(hasLeavesIndexedFrom(t, 0));
-        // assert(hasLeavesIndexedFrom(old(t), 0));
-        // assert(1 <= |p| <= height(t));
-        // assert(count < |leavesIn(t)| == |leavesIn(old(t))| );
-        // leftSiblingsInEquivTrees2(p, old(t), t, count, f, 0);
-
-        // //  Show that value is nodeAt(p, t).v
-        // leafAtPathIsIntValueOfPath(p, t, count, 0);
-        // assert(nodeAt(p, t).v == leavesIn(t)[count].v == value);
-        // //  This proves that t has same siblings as old(t) for path p.
-        // computeRootLeftRightIsCorrectForTree(p, t, branch, zeroes, f, value);
-
-        //   //  compute root value
-        //     r := computeRootLeftRight(p, branch, zeroes, f, value);
-
-        // assert(t.v == r);
-
-        //     //   update path 
-        //     //   as p is to non last leaf it must have a zero and nextPath 
-        //     //   can be computed
+        //     p :=  nextPath(p);
             
-        //     pathToNoLasthasZero(p);
-        //     nextPathIsSucc(p);
-        //     assert(bitListToNat(nextPath(p)) == bitListToNat(p) + 1 == count + 1);
-        //     p := nextPath(p);
+        //     ghost var x := computeLeftSiblingsOnNextpathWithIndex(TREE_HEIGHT, count, old(branch), zero_h, f, v);
+        //     //  Compute left siblings on next path to (count + 1)-th leaf. 
+        //     branch := computeLeftSiblingsOnNextpathWithIndex(TREE_HEIGHT, count, branch, zero_h, f, v);
+        //     assert(branch == x
+        //         // computeLeftSiblingsOnNextpathWithIndex(TREE_HEIGHT, count, old(branch), zero_h, f, v)
+        //         == computeLeftSiblingOnNextPathFromLeftRight(natToBitList(count, TREE_HEIGHT), old(branch), zero_h, f, v)
+        //     );
+        //     //
+            
+
         //     count := count + 1;
-
-        //     //  p is still the path to leaf at index count
-        //     bitToNatToBitsIsIdentity(count, TREE_HEIGHT);
-        //     assert(bitListToNat(p) == count);
-
-        //     //  Prove that right siblings of new path are still zeroes
-        //     rightSiblingsOfLastPathAreDefault(p, t, count, f, 0, d, zeroes);
-
-        //     assert(t.v == r);
-
+        //     assert(count == old(count) + 1);
+        //     assert(old(count) < power2(TREE_HEIGHT) - 1);
+        //     assert(count ==  old(count) + 1 < power2(TREE_HEIGHT) - 1 + 1);
+        //     assert(p ==  nextPath(old(p)));
+        //     pathToSucc(old(p), old(count), TREE_HEIGHT);
+        //     assert(p == natToBitList(count, TREE_HEIGHT));
             
+        //     //  branch is left siblings on path to count
+        //     // assert();
+        //     // assert (forall i :: 0 <= i < |p| && p[i] == 1 ==> 
+        //     //         siblingValueAt(p, t, i + 1) == branch[i]);
+        // }
+
+
+        method get_deposit_root() returns (h_root: T) 
+            requires Valid()
+            requires count < power2(TREE_HEIGHT) - 1 
+
+            // ensures count == 0 ==> h_root == t.v 
+        {
+            //  Show that d == nodeAt(p, t).v
+            // calc == {
+            //     nodeAt(p, t).v;
+            //     leavesIn(t)[natToBitList2(count, h)].v;
+
+            // }
+            // assume(d == nodeAt(p, t).v);
+            // assert(bitListToNat(p) == count);
+            // bitToNatToBitsIsIdentity(count, TREE_HEIGHT);
+            // assert(p == natToBitList(count, TREE_HEIGHT));
+
+            // reveal_siblingValueAt();
+            // computeRootLeftRightUpIsCorrectForTree(p, t, branch, zero_h, f, d);
+ 
+            //  Compute the root using the left siblings on next path (branch) and default value d.
+            h_root := computeRootLeftRightUpWithIndex(TREE_HEIGHT, count, branch, zero_h, f, d);
+            // assert(
+            //     computeRootLeftRightUpWithIndex(TREE_HEIGHT, count, branch, zero_h, f, d)
+            //     ==
+            //     computeRootLeftRightUp(natToBitList2(count, TREE_HEIGHT), branch, zero_h, f, d)
+            //     ==
+            //     computeRootLeftRightUp(p, branch, zero_h, f, d)
+
+            // );
+            // assert(t.v == computeRootLeftRightUp(p, branch, zero_h, f, d));
+        }
+
+        
+
+        /**
+         *  Deposit a value i.e update the state.
+         */
+        // method deposit2(value : T) 
+        //     requires Valid()
+        //     requires count < power2(TREE_HEIGHT) - 1 
+
+        //     modifies this 
+        // {
+            //  Update ghost variables that simulate what is happening on the Merkle tree.
+            //  Add value to tree 
+            // values := values + [value];
+            // assert(|values| == count + 1 < power2(TREE_HEIGHT));
+            // t := buildMerkle(values, TREE_HEIGHT, f, d);
+            // assert(height(t) == TREE_HEIGHT);
+            // assert(isMerkle(t, values, f, d));
+
+            // nextPathSameSiblingsInNextList(TREE_HEIGHT, old(values), value, old(t), t, f, d, p, nextPath(p));
+            // r := computeRootLeftRightUpWithIndex(TREE_HEIGHT, count + 1, branch, zero_h, f, value);
+            // computeWithIndexFromZeroIsCorrect(TREE_HEIGHT, count, branch, zero_h, f, value);
+            // computeRootLeftRightIsCorrectForTree(natToBitList(count, TREE_HEIGHT), t, branch, zero_h, f, value);
+            // assert(r == t.v);            
+
+            // //  Compute nextPath
+            // //  We have to show p (path to count-th leaf, has a zero
+            // assert(bitListToNat(p) == count < power2(TREE_HEIGHT) - 1 == power2(|p|) - 1);
+            // pathToNoLasthasZero(p);
+            // p := nextPath(p);
+            // //  p is path to (count + 1)-th leaf
+            // nextPathIffSucc(old(p), p);
+            // assert(bitListToNat(p) == bitListToNat(old(p)) + 1 == count + 1);
+            // leafAtPathIsIntValueOfPath(p, t, count + 1 , 0);
+            // assert(nodeAt(p, t) == leavesIn(t)[count + 1]);
+
+            // computeLeftSiblingOnNextPathFromLeftRightIsCorrectInATree(natToBitList(count + 1, TREE_HEIGHT), t, branch, zero_h, f, value, count);
+
+           
+            //  Depsoit contract algorithm
+            //  Compute left siblings on next path to (count + 1_th leaf. 
+            // branch := computeLeftSiblingsOnNextpathWithIndex(TREE_HEIGHT, count, branch, zero_h, f, value);
+            // count := count + 1;
+
+            // assert();
+
+            //  branch is the value of siblings on next path.
+            // assert(branch == computeLeftSiblingOnNextPathFromLeftRight(natToBitList(count, TREE_HEIGHT), left, zero_h, f, value));
+            
+            // computeLeftSiblingOnNextPathFromLeftRight();
         // }
 
     }
